vale/code/arch/x64/Views.fst
@@ -23,47 +23,18 @@ let inverses32 (u:unit) =
     assert (Seq.equal x (put32 (get32 x)))
   in Classical.forall_intro aux
 
-private
-abstract
-let get64_def_alt (s:Seq.lseq U8.t 8) : GTot UInt64.t =
-  let open FStar.Mul in
-  let s0 = Seq.slice s 0 4 in
-  let u0 = get32_def s0 in
-  let s1 = Seq.slice s 4 8 in
-  let u1 = get32_def s1 in
-  UInt64.uint_to_t (UInt32.v u0 +
-                    UInt32.v u1 * 0x100000000)
-
-let get64_def_alt_equiv (s:Seq.lseq U8.t 8)
-  : Lemma (get64_def s == get64_def_alt s)
-  = ()
-
-let inverses64_def_aux (x:UInt64.t)
-  : Lemma (get64_def (put64_def x) == x)
-  = ()
-
-#reset-options "--z3rlimit 30"
-let inverses64_def_aux' (x:Seq.lseq U8.t 8)
-  : Lemma (put64_def (get64_def x) `Seq.equal` x)
-  = reveal_opaque get32_def;
-    reveal_opaque put32_def;
-    inverses32();
-    get64_def_alt_equiv x;
-    get64_def_alt_equiv (put64_def (get64_def x));
-    inverses64_def_aux (get64_def x)
-
 #reset-options "--z3rlimit 20"
 let inverses64 (u:unit) =
   reveal_opaque get64_def;
   reveal_opaque put64_def;
-  Classical.forall_intro inverses64_def_aux;
-  Classical.forall_intro inverses64_def_aux'
+  Classical.forall_intro Arch.Types.le_nat64_to_bytes_to_nat64;
+  Classical.forall_intro Arch.Types.le_bytes_to_nat64_to_bytes
 
 let inverses128 (u:unit) =
   reveal_opaque get128_def;
   reveal_opaque put128_def;
-  Classical.forall_intro  Arch.Types.le_quad32_to_bytes_to_quad32;
-  Classical.forall_intro  Arch.Types.le_bytes_to_quad32_to_bytes
+  Classical.forall_intro Arch.Types.le_quad32_to_bytes_to_quad32;
+  Classical.forall_intro Arch.Types.le_bytes_to_quad32_to_bytes
 
 let get32_128_aux1 (x: Seq.lseq U32.t 4): Lemma (put32_128 (get32_128 x) == x) =
   reveal_opaque put32_128_def;
